scheduler/SchTactics.v
@@ -153,6 +153,68 @@ Ltac sch_yield_ii :=
   norm_r; iApply wsim_yield_tgt;
   [right; right; esplits; [refl|..]; et; set_solver|et|et|sch_auto; [..|try sch_intros]].
 
+Lemma unfold_img_lat `{Σ:GRA} peeking fsp lbody body arg:
+  img_lat peeking fsp lbody body arg =
+    r <- img_lat_body peeking fsp lbody body arg;;
+    match r with
+    | inl _ => tau;; img_lat peeking fsp lbody body arg
+    | inr r => Ret r
+    end.
+Proof.
+  rewrite /img_lat. erewrite -> (bisim_is_eq (unfold_iter _ _)) at 1.
+  f_equal. extensionalities. destruct H; et.
+  repeat f_equal. destruct u; et.
+Qed.
+
+Lemma unfold_real_lat `{Σ:GRA} peeking fsp lbody body arg:
+  real_lat peeking fsp lbody body arg =
+    r <- real_lat_body peeking fsp lbody body arg;;
+    match r with
+    | inl _ => tau;; real_lat peeking fsp lbody body arg
+    | inr r => Ret r
+    end.
+Proof.
+  rewrite /real_lat. erewrite -> (bisim_is_eq (unfold_iter _ _)) at 1.
+  f_equal. extensionalities. destruct H; et.
+  repeat f_equal. destruct u; et.
+Qed.
+
+Ltac unfold_img_lat_l :=
+  let marker := fresh "MARKER" in
+  set_marker marker;
+  hide_ihyps;
+  only_itree_l;
+  rewrite {1}unfold_img_lat {1}/img_lat_body;
+  show_until marker;
+  steps_l.
+
+Ltac unfold_img_lat_r :=
+  let marker := fresh "MARKER" in
+  set_marker marker;
+  hide_ihyps;
+  only_itree_r;
+  rewrite {1}unfold_img_lat {1}/img_lat_body;
+  show_until marker;
+  steps_r.
+
+Ltac unfold_real_lat_l :=
+  let marker := fresh "MARKER" in
+  set_marker marker;
+  hide_ihyps;
+  only_itree_l;
+  rewrite {1}unfold_real_lat {1}/real_lat_body;
+  show_until marker;
+  steps_l.
+
+Ltac unfold_real_lat_r :=
+  let marker := fresh "MARKER" in
+  set_marker marker;
+  hide_ihyps;
+  only_itree_r;
+  rewrite {1}unfold_real_lat {1}/real_lat_body;
+  show_until marker;
+  steps_r.
+
 Section RealLAT.
   Context `{CRIS: !crisG Γ Σ α β τ _S _I}.
   Context `{SCH: !schG}.
@@ -168,16 +230,14 @@ Section RealLAT.
 
   Local Notation sim Ep r g := (wsim fl_s fl_t Ist Ep r g R_s R_t).
 
-  Lemma wsim_real_lat_both (peeking: bool)
+  Lemma wsim_real_lat_both
     fsp_s fsp_t body_s body_t arg_s arg_t k_s k_t
     img_s img_t (msk_s msk_t: _ → bool) scp_s scp_t
     :
     msk_s SchHdr.yield →
     msk_t SchHdr.yield →
     Ist st_s st_t ∗
-    (if peeking
-     then (□ ∀ x_s, ∃ x_t, precondS fsp_s x_s arg_s ==∗ precondS fsp_t x_t arg_t ∗ (precondS fsp_t x_t arg_t ==∗ precondS fsp_s x_s arg_s))
-     else emp) ∗
+    (□ ∀ x_s, ∃ x_t, precondS fsp_s x_s arg_s ==∗ precondS fsp_t x_t arg_t ∗ (precondS fsp_t x_t arg_t ==∗ precondS fsp_s x_s arg_s)) ∗
     (∀ st_src st_tgt,
       Ist st_src st_tgt -∗ 
       sim (∅,∅) r g RR true true
@@ -189,18 +249,18 @@ Section RealLAT.
                    Ret ret_t)) >>= k_t))
     ⊢
     sim (∅,∅) r g RR ps pt
-      (st_s, SB.sandbox img_s msk_s scp_s (SModTr.trans sp_none (real_lat peeking fsp_s 𝒴 body_s arg_s)) >>= k_s)
-      (st_t, SB.sandbox img_t msk_t scp_t (SModTr.trans sp_none (real_lat peeking fsp_t 𝒴 body_t arg_t)) >>= k_t).
+      (st_s, SB.sandbox img_s msk_s scp_s (SModTr.trans sp_none (real_lat true fsp_s 𝒴 body_s arg_s)) >>= k_s)
+      (st_t, SB.sandbox img_t msk_t scp_t (SModTr.trans sp_none (real_lat true fsp_t 𝒴 body_t arg_t)) >>= k_t).
   Proof using SCH.
     i. iIntros "H". iApply wsim_reset. iStopProof.
     revert st_s. combine_quant st_t.
     eapply wsim_coind. intros g' Hg CIH [st_t st_s].
     iIntros "[IST [#COND SIM]] /=". destruct_quant CIH.
-    
-    rewrite /real_lat. unfold_iter_l. steps_l. unfold_iter_r. steps_r.
+
+    unfold_real_lat_l. unfold_real_lat_r.
     sch_yield_rr. sch_yield_l.
     steps_r. force_l _q. steps_l.
-    destruct (peeking && _q) eqn: E; cycle 1; steps_l; steps_r.
+    destruct _q eqn: E; cycle 1; steps_l; steps_r.
     { iApply wsim_mono_knowledge; cycle 2.
       { eapply eq_ind. iApply ("SIM" with "IST").
         rewrite !SRed.bind !SBRed.bind !bind_bind.
@@ -233,7 +293,7 @@ Section RealLAT.
   Unshelve. all: exact 0.
   Qed.
 
-  Lemma wsim_real_lat_tgt (peeking: bool)
+  Lemma wsim_real_lat_tgt
     fsp_t body_t x_t arg_t E tid_res q my_tid
     k_s k_t img_s img_t (msk_s msk_t: _ → bool) scp_s scp_t sp_s
     I
@@ -248,11 +308,10 @@ Section RealLAT.
     msk_s SchHdr.yield →
     msk_t SchHdr.yield →
     I ∗ Ist st_s st_t ∗ (if tid_res then SchAS.tid_user q my_tid else emp) ∗
-    (if peeking
-     then □ (∀ st_src st_tgt,
+    (□ (∀ st_src st_tgt,
        I -∗ winv (E, E) -∗ Ist st_src st_tgt -∗ (if tid_res then SchAS.tid_user q my_tid else emp) ==∗
        precondS fsp_t x_t arg_t ∗ (precondS fsp_t x_t arg_t ==∗ I ∗ winv (E, E) ∗ Ist st_src st_tgt ∗ (if tid_res then SchAS.tid_user q my_tid else emp)))
-     else emp) ∗
+    ) ∗
     (∀ st_src st_tgt,
      I -∗ Ist st_src st_tgt -∗ (if tid_res then SchAS.tid_user q my_tid else emp) -∗
      sim (E,E) r g RR true true
@@ -263,17 +322,17 @@ Section RealLAT.
     ⊢
     sim (E,E) r g RR ps pt
       (st_s, SB.sandbox img_s msk_s scp_s (SModTr.trans sp_s 𝒴) >>= k_s)
-      (st_t, SB.sandbox img_t msk_t scp_t (SModTr.trans sp_none (real_lat peeking fsp_t 𝒴 body_t arg_t)) >>= k_t).
+      (st_t, SB.sandbox img_t msk_t scp_t (SModTr.trans sp_none (real_lat true fsp_t 𝒴 body_t arg_t)) >>= k_t).
   Proof using.
     i. iIntros "H". iApply wsim_reset. iStopProof.
     revert st_s. combine_quant st_t.
     eapply wsim_coind. intros g' Hg CIH [st_t st_s].
     iIntros "[I [IST [TID [#COND SIM]]]] /=". destruct_quant CIH.
 
-    rewrite /real_lat. unfold_iter_r. steps_r.
+    unfold_real_lat_r.
     iApply wsim_yield_tgt; [|et|et|try (sch_auto; sch_intros)].
     { des; subst; [left|right;left]; et. }
-    steps_r. destruct (peeking && _q) eqn: E0; cycle 1; steps_r.
+    steps_r. destruct _q eqn: E0; cycle 1; steps_r.
     { iApply wsim_mono_knowledge; cycle 2.
       { eapply eq_ind. iApply ("SIM" with "I IST TID").
         rewrite !SRed.bind !SBRed.bind !bind_bind.
