theories/simulations/msim/TacticsInit.v
@@ -78,9 +78,9 @@ Ltac init_sim :=
 
 Ltac iinit_simF := initialize_simF.
 
-Ltac prove_fr_to_img :=
-  iinit_simF; iDestruct "IST" as "->"; iIntros "_"; istep_r;
-  match goal with |- context[real_lat ?peeking ?fsp _] =>
-    iApply (isim_fr_to_img peeking fsp)
-  end;
-  rewrite !SRed.core !SBRed.choose; refl.
+(* Ltac prove_real_to_img := *)
+(*   iinit_simF; iDestruct "IST" as "->"; iIntros "_"; istep_r; *)
+(*   match goal with |- context[real_lat ?peeking ?fsp] => *)
+(*     iApply (isim_lat_real_to_img peeking fsp) *)
+(*   end; *)
+(*   rewrite !SRed.core !SBRed.choose; refl. *)
